theory/Util/Rel.v
@@ -1,6 +1,0 @@
-
-Fixpoint Rel (n : nat) (X : Type) : Type :=
-  match n with
-  | 0 => Prop
-  | S m => X -> Rel m X
-  end.
